# baseURI: https://data.nasa.gov/ontologies/atmonto/flightInst
# imports: https://data.nasa.gov/ontologies/atmonto/ATM

@prefix atm: <https://data.nasa.gov/ontologies/atmonto/ATM#> .
@prefix data: <https://data.nasa.gov/ontologies/atmonto/data#> .
@prefix doc: <https://data.nasa.gov/ontologies/atmonto/documentation#> .
@prefix eqp: <https://data.nasa.gov/ontologies/atmonto/equipment#> .
@prefix gen: <https://data.nasa.gov/ontologies/atmonto/general#> .
@prefix nas: <https://data.nasa.gov/ontologies/atmonto/NAS#> .
@prefix owl: <http://www.w3.org/2002/07/owl#> .
@prefix rdf: <http://www.w3.org/1999/02/22-rdf-syntax-ns#> .
@prefix rdfs: <http://www.w3.org/2000/01/rdf-schema#> .
@prefix xml: <http://www.w3.org/XML/1998/namespace> .
@prefix xsd: <http://www.w3.org/2001/XMLSchema#> .

<https://data.nasa.gov/ontologies/atmonto/flightInst> a owl:Ontology ;
    owl:imports <https://data.nasa.gov/ontologies/atmonto/ATM> .


## Flights #############################################################

atm:actualArrivalDay a owl:FunctionalProperty,
        owl:ObjectProperty ;
    rdfs:label "actual arrival day" ;
    rdfs:comment "Links a flight with the day on which the flight arrives. This is the day determined by surveillance data sources to be the 'actual' day of arrival, versus the scheduled day or the day specified in the flight plan, etc." ;
    rdfs:domain atm:Flight ;
    rdfs:range nas:NASday .

atm:actualArrivalTime a owl:DatatypeProperty,
        owl:FunctionalProperty ;
    rdfs:label "actual arrival time" ;
    rdfs:comment "The time determined by surveillance data sources to be the 'actual' time of flight arrival, versus the scheduled time or the time specified in the flight plan, etc." ;
    rdfs:domain atm:Flight ;
    rdfs:range xsd:dateTime .

atm:actualDepartureDay a owl:FunctionalProperty,
        owl:ObjectProperty ;
    rdfs:label "actual departure day" ;
    rdfs:comment "Links a flight with the day on which the flight departs. This is the day determined by surveillance data sources to be the 'actual' day of departure, versus the scheduled day or the day specified in the flight plan, etc." ;
    rdfs:domain atm:Flight ;
    rdfs:range nas:NASday .

atm:actualDepartureTime a owl:DatatypeProperty,
        owl:FunctionalProperty ;
    rdfs:label "actual departure time" ;
    rdfs:comment "The time determined by surveillance data sources to be the 'actual' time of flight departure, versus the scheduled time or the time specified in the flight plan, etc." ;
    rdfs:domain atm:Flight ;
    rdfs:range xsd:dateTime .

atm:aircraftTypeFlown a owl:FunctionalProperty,
        owl:ObjectProperty ;
    rdfs:label "aircraft type flown" ;
    rdfs:comment "Links a flight with the type of aircraft flown. The aircraft 'type' corresponds to a set of aircraft models with similar characteristics." ;
    rdfs:domain atm:Flight ;
    rdfs:range eqp:AircraftType .

atm:Flight a owl:Class ;
    rdfs:label "Flight" ;
    rdfs:comment "A single flight segment from origin to destination." ;
    rdfs:subClassOf [ a owl:Restriction ;
            owl:allValuesFrom [ a rdfs:Datatype ;
                    owl:oneOf [ a rdf:List ;
                            rdf:first "Air Taxi" ;
                            rdf:rest [ a rdf:List ;
                                    rdf:first "Cargo" ;
                                    rdf:rest [ a rdf:List ;
                                            rdf:first "Commercial" ;
                                            rdf:rest [ a rdf:List ;
                                                    rdf:first "GA" ;
                                                    rdf:rest [ a rdf:List ;
                                                            rdf:first "Military" ;
                                                            rdf:rest () ] ] ] ] ] ] ;
            owl:onProperty atm:userCategory ],
        owl:Thing .

atm:arrivalAirport a owl:FunctionalProperty,
        owl:ObjectProperty ;
    rdfs:label "arrival airport" ;
    rdfs:comment "Links to the actual arrival airport for the flight." ;
    rdfs:domain atm:Flight ;
    rdfs:range nas:Airport .

atm:callSign a owl:DatatypeProperty ;
    rdfs:label "call sign" ;
    rdfs:comment "The flight identifier (3-letter ICAO code plus number)." ;
    rdfs:domain atm:Flight ;
    rdfs:range xsd:string .

atm:departureAirport a owl:FunctionalProperty,
        owl:ObjectProperty ;
    rdfs:label "departure airport" ;
    rdfs:comment "Links to the actual departure airport for the flight." ;
    rdfs:domain atm:Flight ;
    rdfs:range nas:Airport .

atm:hasActualRoute a owl:FunctionalProperty,
        owl:ObjectProperty ;
    rdfs:label "has actual route" ;
    rdfs:comment "Links a flight to its actual trajectory (i.e., a sequence of track points), as determined by flight track surveillance data." ;
    rdfs:domain atm:Flight ;
    rdfs:range atm:ActualFlightRoute .

atm:hasPlannedRoute a owl:ObjectProperty ;
    rdfs:label "has planned route" ;
    rdfs:comment "Links a flight to a version of its flight plan. (Which version gets stored is application-dependent.) There are multiple versions of the flight plan generated and then amended during the course of the flight, starting in the pre-flight timeframe and extending through to the termination of the flight." ;
    rdfs:domain atm:Flight ;
    rdfs:range atm:PlannedFlightRoute .

atm:operatedBy a owl:FunctionalProperty,
        owl:ObjectProperty ;
    rdfs:label "operated by" ;
    rdfs:comment "Links a flight to its carrier airline." ;
    rdfs:domain atm:Flight ;
    rdfs:range nas:AirCarrier .

atm:userCategory a owl:DatatypeProperty,
        owl:FunctionalProperty ;
    rdfs:label "user category" ;
    rdfs:comment "The type of airspace user that this flight represents: GA, Air Taxi, Cargo, Commercial, Military. Also used to constrain a flight specification to contain only flights representing a specific user category." ;
    rdfs:domain [ a owl:Class ;
            owl:unionOf ( atm:Flight atm:FlightSpec ) ] ;
    rdfs:range xsd:string .

atm:aircraftFlown a owl:FunctionalProperty,
        owl:ObjectProperty ;
    rdfs:label "aircraft flown" ;
    rdfs:comment "Links a flight with the actual aircraft used." ;
    rdfs:domain atm:Flight ;
    rdfs:range eqp:Aircraft .

atm:AAL100-201407150030 a atm:Flight ;
    rdfs:label "Flight AAL100 on 2014-07-15 00:30:00"^^xsd:string ;
    atm:actualArrivalDay nas:Day20140715 ;
    atm:actualArrivalTime "2014-07-15T02:46:47"^^xsd:dateTime ;
    atm:actualDepartureDay nas:Day20140715 ;
    atm:actualDepartureTime "2014-07-15T00:30:00"^^xsd:dateTime ;
    atm:aircraftTypeFlown eqp:B77WAircraftType ;
    atm:arrivalAirport nas:EGLLairport ;
    atm:callSign "AAL100"^^xsd:string ;
    atm:departureAirport nas:KJFKairport ;
    atm:hasActualRoute atm:ActualRouteAAL100-201407150030 ;
    atm:hasPlannedRoute atm:PlannedRouteAAL100-201407150030 ;
    atm:operatedBy nas:AALairline ;
    atm:userCategory "COMMERCIAL"^^xsd:string .

atm:AAL1102-201407150046 a atm:Flight ;
    rdfs:label "Flight AAL1102 on 2014-07-15 00:46:00"^^xsd:string ;
    atm:actualArrivalDay nas:Day20140715 ;
    atm:actualArrivalTime "2014-07-15T03:13:00"^^xsd:dateTime ;
    atm:actualDepartureDay nas:Day20140715 ;
    atm:actualDepartureTime "2014-07-15T00:46:00"^^xsd:dateTime ;
    atm:aircraftFlown eqp:AircraftN963AN ;
    atm:aircraftTypeFlown eqp:B738AircraftType ;
    atm:arrivalAirport nas:KMIAairport ;
    atm:callSign "AAL1102"^^xsd:string ;
    atm:departureAirport nas:KLGAairport ;
    atm:hasActualRoute atm:ActualRouteAAL1102-201407150046 ;
    atm:hasPlannedRoute atm:PlannedRouteAAL1102-201407150046 ;
    atm:operatedBy nas:AALairline ;
    atm:userCategory "COMMERCIAL"^^xsd:string .

atm:AAL1144-201407150040 a atm:Flight ;
    rdfs:label "Flight AAL1144 on 2014-07-15 00:40:00"^^xsd:string ;
    atm:actualArrivalDay nas:Day20140715 ;
    atm:actualArrivalTime "2014-07-15T04:01:00"^^xsd:dateTime ;
    atm:actualDepartureDay nas:Day20140715 ;
    atm:actualDepartureTime "2014-07-15T00:40:00"^^xsd:dateTime ;
    atm:aircraftFlown eqp:AircraftN942NN ;
    atm:aircraftTypeFlown eqp:B738AircraftType ;
    atm:arrivalAirport nas:KDFWairport ;
    atm:callSign "AAL1144"^^xsd:string ;
    atm:departureAirport nas:KLGAairport ;
    atm:hasActualRoute atm:ActualRouteAAL1144-201407150040 ;
    atm:hasPlannedRoute atm:PlannedRouteAAL1144-201407150040 ;
    atm:operatedBy nas:AALairline ;
    atm:userCategory "COMMERCIAL"^^xsd:string .

atm:AAL1170-201407150053 a atm:Flight ;
    rdfs:label "Flight AAL1170 on 2014-07-15 00:53:00"^^xsd:string ;
    atm:actualArrivalDay nas:Day20140715 ;
    atm:actualArrivalTime "2014-07-15T03:37:00"^^xsd:dateTime ;
    atm:actualDepartureDay nas:Day20140715 ;
    atm:actualDepartureTime "2014-07-15T00:53:00"^^xsd:dateTime ;
    atm:aircraftFlown eqp:AircraftN871NN ;
    atm:aircraftTypeFlown eqp:B738AircraftType ;
    atm:arrivalAirport nas:KLGAairport ;
    atm:callSign "AAL1170"^^xsd:string ;
    atm:departureAirport nas:KDFWairport ;
    atm:hasActualRoute atm:ActualRouteAAL1170-201407150053 ;
    atm:hasPlannedRoute atm:PlannedRouteAAL1170-201407150053 ;
    atm:operatedBy nas:AALairline ;
    atm:userCategory "COMMERCIAL"^^xsd:string .

atm:AAL20-201407152358 a atm:Flight ;
    rdfs:label "Flight AAL20 on 2014-07-15 23:58:00"^^xsd:string ;
    atm:actualArrivalDay nas:Day20140716 ;
    atm:actualArrivalTime "2014-07-16T04:54:00"^^xsd:dateTime ;
    atm:actualDepartureDay nas:Day20140715 ;
    atm:actualDepartureTime "2014-07-15T23:58:00"^^xsd:dateTime ;
    atm:aircraftFlown eqp:AircraftN784AA ;
    atm:aircraftTypeFlown eqp:A321AircraftType ;
    atm:arrivalAirport nas:KJFKairport ;
    atm:callSign "AAL20"^^xsd:string ;
    atm:departureAirport nas:KSFOairport ;
    atm:hasActualRoute atm:ActualRouteAAL20-201407152358 ;
    atm:hasPlannedRoute atm:PlannedRouteAAL20-201407152358 ;
    atm:operatedBy nas:AALairline ;
    atm:userCategory "COMMERCIAL"^^xsd:string .

atm:ACA722-201407150025 a atm:Flight ;
    rdfs:label "Flight ACA722 on 2014-07-15 00:25:00"^^xsd:string ;
    atm:actualArrivalDay nas:Day20140715 ;
    atm:actualArrivalTime "2014-07-15T01:19:00"^^xsd:dateTime ;
    atm:actualDepartureDay nas:Day20140715 ;
    atm:actualDepartureTime "2014-07-15T00:25:00"^^xsd:dateTime ;
    atm:arrivalAirport nas:KLGAairport ;
    atm:callSign "ACA722"^^xsd:string ;
    atm:departureAirport nas:CYYZairport ;
    atm:hasActualRoute atm:ActualRouteACA722-201407150025 ;
    atm:hasPlannedRoute atm:PlannedRouteACA722-201407150025 ;
    atm:operatedBy nas:ACAairline ;
    atm:userCategory "COMMERCIAL"^^xsd:string .

atm:ASA14-201407150005 a atm:Flight ;
    rdfs:label "Flight ASA14 on 2014-07-15 00:05:00"^^xsd:string ;
    atm:actualArrivalDay nas:Day20140715 ;
    atm:actualArrivalTime "2014-07-15T04:49:00"^^xsd:dateTime ;
    atm:actualDepartureDay nas:Day20140715 ;
    atm:actualDepartureTime "2014-07-15T00:05:00"^^xsd:dateTime ;
    atm:aircraftFlown eqp:AircraftN413AS ;
    atm:aircraftTypeFlown eqp:B739AircraftType ;
    atm:arrivalAirport nas:KEWRairport ;
    atm:callSign "ASA14"^^xsd:string ;
    atm:departureAirport nas:KSEAairport ;
    atm:hasActualRoute atm:ActualRouteASA14-201407150005 ;
    atm:hasPlannedRoute atm:PlannedRouteASA14-201407150005 ;
    atm:operatedBy nas:ASAairline ;
    atm:userCategory "COMMERCIAL"^^xsd:string .

atm:ASQ3831-201407150019 a atm:Flight ;
    rdfs:label "Flight ASQ3831 on 2014-07-15 00:19:00"^^xsd:string ;
    atm:actualArrivalDay nas:Day20140715 ;
    atm:actualArrivalTime "2014-07-15T01:22:00"^^xsd:dateTime ;
    atm:actualDepartureDay nas:Day20140715 ;
    atm:actualDepartureTime "2014-07-15T00:19:00"^^xsd:dateTime ;
    atm:arrivalAirport nas:KEWRairport ;
    atm:callSign "ASQ3831"^^xsd:string ;
    atm:departureAirport nas:CYYZairport ;
    atm:hasActualRoute atm:ActualRouteASQ3831-201407150019 ;
    atm:hasPlannedRoute atm:PlannedRouteASQ3831-201407150019 ;
    atm:operatedBy nas:ASQairline ;
    atm:userCategory "COMMERCIAL"^^xsd:string .

atm:ASQ4423-201407150037 a atm:Flight ;
    rdfs:label "Flight ASQ4423 on 2014-07-15 00:37:00"^^xsd:string ;
    atm:actualArrivalDay nas:Day20140715 ;
    atm:actualArrivalTime "2014-07-15T01:33:00"^^xsd:dateTime ;
    atm:actualDepartureDay nas:Day20140715 ;
    atm:actualDepartureTime "2014-07-15T00:37:00"^^xsd:dateTime ;
    atm:aircraftFlown eqp:AircraftN11548 ;
    atm:aircraftTypeFlown eqp:E145AircraftType ;
    atm:arrivalAirport nas:KEWRairport ;
    atm:callSign "ASQ4423"^^xsd:string ;
    atm:departureAirport nas:KMHTairport ;
    atm:hasActualRoute atm:ActualRouteASQ4423-201407150037 ;
    atm:hasPlannedRoute atm:PlannedRouteASQ4423-201407150037 ;
    atm:operatedBy nas:ASQairline ;
    atm:userCategory "COMMERCIAL"^^xsd:string .

atm:CHQ2945-201407150047 a atm:Flight ;
    rdfs:label "Flight CHQ2945 on 2014-07-15 00:47:00"^^xsd:string ;
    atm:actualArrivalDay nas:Day20140715 ;
    atm:actualArrivalTime "2014-07-15T02:27:00"^^xsd:dateTime ;
    atm:actualDepartureDay nas:Day20140715 ;
    atm:actualDepartureTime "2014-07-15T00:47:00"^^xsd:dateTime ;
    atm:aircraftTypeFlown eqp:E145AircraftType ;
    atm:arrivalAirport nas:KCLTairport ;
    atm:callSign "CHQ2945"^^xsd:string ;
    atm:departureAirport nas:KJFKairport ;
    atm:hasActualRoute atm:ActualRouteCHQ2945-201407150047 ;
    atm:hasPlannedRoute atm:PlannedRouteCHQ2945-201407150047 ;
    atm:operatedBy nas:CHQairline ;
    atm:userCategory "AIR TAXI"^^xsd:string .

## Aircraft ############################################################

eqp:Aircraft a owl:Class ;
    rdfs:label "Aircraft" ;
    rdfs:comment "A physical realization of an aircraft, produced according to the specifications defined for a specific model type." ;
    rdfs:subClassOf [ a owl:Restriction ;
            owl:allValuesFrom nas:AirframeManufacturer ;
            owl:onProperty eqp:manufacturedBy ],
        eqp:DecomposableSystem,
        gen:SequencedItem .

eqp:aircraftModelCertainty a owl:DatatypeProperty,
        owl:FunctionalProperty ;
    rdfs:label "aircraft model certainty" ;
    rdfs:comment "A numeric measure between 0 and 1 reflecting how certain the eqp:hasAircraftModel link is to be correct between the aircraft and the model. A value of one indicates 100% certainty. A lesser value is not to be taken as a percentage, but is a heuristic similarity value taken from the scoring of the TF/IDF similarity assessment performed between the FAA aircraft make/model in the FAA registration database and ICAO make/model names used in the ontology." ;
    rdfs:domain eqp:Aircraft ;
    rdfs:range xsd:float .

eqp:aircraftRegistrant a owl:DatatypeProperty ;
    rdfs:label "aircraft registrant" ;
    rdfs:comment "The name of the entity that registered the aircraft with the FAA." ;
    rdfs:domain eqp:Aircraft ;
    rdfs:range xsd:string .

eqp:aircraftSerialNumber a owl:DatatypeProperty,
        owl:FunctionalProperty ;
    rdfs:label "serial number" ;
    rdfs:comment "The manufacturer serial number of the aircraft." ;
    rdfs:domain eqp:Aircraft ;
    rdfs:range xsd:string .

eqp:certificateIssueDate a owl:DatatypeProperty,
        owl:FunctionalProperty ;
    rdfs:label "certificate issue date" ;
    rdfs:comment "The date that an operating certificate was issued to the aircraft." ;
    rdfs:domain eqp:Aircraft ;
    rdfs:range xsd:date .

eqp:hasAircraftModel a owl:FunctionalProperty,
        owl:ObjectProperty ;
    rdfs:label "has aircraft model" ;
    rdfs:comment "Links a specific aircraft to its model." ;
    rdfs:domain eqp:Aircraft ;
    rdfs:range eqp:AircraftModel .

eqp:manufactureYear a owl:DatatypeProperty,
        owl:FunctionalProperty ;
    rdfs:label "manufacture year" ;
    rdfs:comment "The year the system was manufactured." ;
    rdfs:domain eqp:EngineeredSystem ;
    rdfs:range xsd:integer .

eqp:modeSCode a owl:DatatypeProperty,
        owl:FunctionalProperty ;
    rdfs:label "mode SCode" ;
    rdfs:comment "The unique Mode S address of the transponder aboard the aircraft. Mode S equipment on aircraft are assigned a unique ICAO 24-bit address or (informally) Mode S hex code upon national registration and this address becomes a part of the aircraft's Certificate of Registration." ;
    rdfs:domain eqp:Aircraft ;
    rdfs:range xsd:string .                    

eqp:numberOfEngines a owl:DatatypeProperty,
        owl:FunctionalProperty ;
    rdfs:label "number of engines" ;
    rdfs:comment "The number of engines specified for this aircraft model or found on this aircraft." ;
    rdfs:domain eqp:Aircraft,
        eqp:AircraftModel ;
    rdfs:range xsd:integer .

eqp:numberOfSeats a owl:DatatypeProperty,
        owl:FunctionalProperty ;
    rdfs:label "number of seats" ;
    rdfs:comment "The number of seats on this aircraft." ;
    rdfs:domain eqp:Aircraft ;
    rdfs:range xsd:integer .

eqp:registrationNumber a owl:DatatypeProperty,
        owl:FunctionalProperty ;
    rdfs:label "registration number" ;
    rdfs:comment "The aircraft FAA registration number (the tail number, or the N-Number in the US)." ;
    rdfs:domain eqp:Aircraft ;
    rdfs:range xsd:string .

eqp:AircraftN963AN a eqp:Aircraft ;
    rdfs:label "Aircraft N963AN"^^xsd:string ;
    eqp:aircraftModelCertainty "1.0000000000000002"^^xsd:float ;
    eqp:aircraftRegistrant "AMERICAN AIRLINES INC"^^xsd:string ;
    eqp:aircraftSerialNumber "29543"^^xsd:string ;
    eqp:certificateIssueDate "2001-05-04"^^xsd:date ;
    eqp:hasAircraftModel eqp:Boeing-737-823 ;
    eqp:manufactureYear 2001 ;
    eqp:modeSCode 53263530 ;
    eqp:numberOfEngines 2 ;
    eqp:numberOfSeats 162 ;
    eqp:registrationNumber "N963AN"^^xsd:string .

eqp:AircraftN942NN a eqp:Aircraft ;
    rdfs:label "Aircraft N942NN"^^xsd:string ;
    eqp:aircraftModelCertainty "1.0000000000000002"^^xsd:float ;
    eqp:aircraftRegistrant "WELLS FARGO BANK NORTHWEST NA TRUSTEE"^^xsd:string ;
    eqp:aircraftSerialNumber "33492"^^xsd:string ;
    eqp:certificateIssueDate "2013-12-30"^^xsd:date ;
    eqp:hasAircraftModel eqp:Boeing-737-823 ;
    eqp:manufactureYear 2013 ;
    eqp:modeSCode 53212717 ;
    eqp:numberOfEngines 2 ;
    eqp:numberOfSeats 162 ;
    eqp:registrationNumber "N942NN"^^xsd:string .

eqp:AircraftN871NN a eqp:Aircraft ;
    rdfs:label "Aircraft N871NN"^^xsd:string ;
    eqp:aircraftModelCertainty "1.0000000000000002"^^xsd:float ;
    eqp:aircraftRegistrant "WILMINGTON TRUST CO TRUSTEE"^^xsd:string ;
    eqp:aircraftSerialNumber "31127"^^xsd:string ;
    eqp:certificateIssueDate "2011-11-14"^^xsd:date ;
    eqp:hasAircraftModel eqp:Boeing-737-823 ;
    eqp:manufactureYear 2011 ;
    eqp:modeSCode 52775506 ;
    eqp:numberOfEngines 2 ;
    eqp:numberOfSeats 162 ;
    eqp:registrationNumber "N871NN"^^xsd:string .

eqp:AircraftN784AA a eqp:Aircraft ;
    rdfs:label "Aircraft N784AA"^^xsd:string ;
    eqp:aircraftModelCertainty "0.9879913721631963"^^xsd:float ;
    eqp:aircraftRegistrant "HAYDEN CHARLES J JR"^^xsd:string ;
    eqp:aircraftSerialNumber "D-6858"^^xsd:string ;
    eqp:certificateIssueDate "1991-02-28"^^xsd:date ;
    eqp:hasAircraftModel eqp:Beech-35-P35 ;
    eqp:manufactureYear 1961 ;
    eqp:modeSCode 52517543 ;
    eqp:numberOfEngines 1 ;
    eqp:numberOfSeats 4 ;
    eqp:registrationNumber "N784AA"^^xsd:string .

eqp:AircraftN413AS a eqp:Aircraft ;
    rdfs:label "Aircraft N413AS"^^xsd:string ;
    eqp:aircraftModelCertainty "1.0"^^xsd:float ;
    eqp:aircraftRegistrant "ALASKA AIRLINES INC"^^xsd:string ;
    eqp:aircraftSerialNumber "35205"^^xsd:string ;
    eqp:certificateIssueDate "2013-03-28"^^xsd:date ;
    eqp:hasAircraftModel eqp:Boeing-737-990ER ;
    eqp:manufactureYear 2013 ;
    eqp:modeSCode 51157526 ;
    eqp:numberOfEngines 2 ;
    eqp:numberOfSeats 222 ;
    eqp:registrationNumber "N413AS"^^xsd:string .

eqp:AircraftN11548 a eqp:Aircraft ;
    rdfs:label "Aircraft N11548"^^xsd:string ;
    eqp:aircraftModelCertainty "1.0"^^xsd:float ;
    eqp:aircraftRegistrant "WELLS FARGO BANK NORTHWEST NA TRUSTEE"^^xsd:string ;
    eqp:aircraftSerialNumber "145565"^^xsd:string ;
    eqp:certificateIssueDate "2002-05-30"^^xsd:date ;
    eqp:hasAircraftModel eqp:Embraer-EMB145-LR ;
    eqp:manufactureYear 2002 ;
    eqp:modeSCode 50040713 ;
    eqp:numberOfEngines 2 ;
    eqp:numberOfSeats 55 ;
    eqp:registrationNumber "N11548"^^xsd:string .

## Aircraft type #######################################################

eqp:AircraftType a owl:Class ;
    rdfs:label "Aircraft Type" ;
    rdfs:comment "An aircraft type represents a set of related aircraft models. Each type corresponds to one of the FAA's aircraft type designators (e.g., B777 covers all Boeing 777 models)." ;
    rdfs:subClassOf owl:Thing .

eqp:aircraftTypeDesignator a owl:DatatypeProperty,
        owl:FunctionalProperty ;
    rdfs:label "aircraft type designator" ;
    rdfs:comment "The type designator code for this type of aircraft (e.g., B777)." ;
    rdfs:domain eqp:AircraftType ;
    rdfs:range xsd:string .

eqp:hasAircraftEngineType a owl:FunctionalProperty,
        owl:ObjectProperty ;
    rdfs:label "has aircraft engine type" ;
    rdfs:comment "Links an aircraft type to the type of engine it uses." ;
    rdfs:domain eqp:AircraftType ;
    rdfs:range eqp:EngineType .

eqp:hasAircraftWeightClass a owl:FunctionalProperty,
        owl:ObjectProperty ;
    rdfs:label "has aircraft weight class" ;
    rdfs:comment "Links an aircraft model to its weight class." ;
    rdfs:domain eqp:AircraftType ;
    rdfs:range eqp:AircraftWeightClass .

eqp:hasAircraftWakeCategory a owl:FunctionalProperty,
        owl:ObjectProperty ;
    rdfs:label "has aircraft wake category" ;
    rdfs:comment "Links an aircraft model to its wake category." ;
    rdfs:domain eqp:AircraftType ;
    rdfs:range eqp:AircraftWakeCategory .

eqp:B77WAircraftType a eqp:AircraftType ;
    rdfs:label "Aircraft Type B77W"^^xsd:string ;
    eqp:aircraftTypeDesignator "B77W"^^xsd:string ;
    eqp:hasAircraftEngineType eqp:JetEngineType ;                       
    eqp:hasAircraftWeightClass eqp:HighAircraftWeightClass ;            
    eqp:numberOfEngines 2 .

eqp:B738AircraftType a eqp:AircraftType ;
    rdfs:label "Aircraft Type B738"^^xsd:string ;
    eqp:aircraftTypeDesignator "B738"^^xsd:string ;
    eqp:hasAircraftEngineType eqp:JetEngineType ;
    eqp:hasAircraftWakeCategory eqp:AircraftWakeCategoryD5 ;
    eqp:hasAircraftWeightClass eqp:MediumAircraftWeightClass ;
    eqp:numberOfEngines 2 .

eqp:A321AircraftType a eqp:AircraftType ;
    rdfs:label "Aircraft Type A321"^^xsd:string ;
    eqp:aircraftTypeDesignator "A321"^^xsd:string ;
    eqp:hasAircraftEngineType eqp:JetEngineType ;
    eqp:hasAircraftWakeCategory eqp:AircraftWakeCategoryD5 ;
    eqp:hasAircraftWeightClass eqp:MediumAircraftWeightClass ;
    eqp:numberOfEngines 2 .

eqp:B739AircraftType a eqp:AircraftType ;
    rdfs:label "Aircraft Type B739"^^xsd:string ;
    eqp:aircraftTypeDesignator "B739"^^xsd:string ;
    eqp:hasAircraftEngineType eqp:JetEngineType ;
    eqp:hasAircraftWakeCategory eqp:AircraftWakeCategoryD5 ;
    eqp:hasAircraftWeightClass eqp:MediumAircraftWeightClass ;
    eqp:numberOfEngines 2 .

eqp:E145AircraftType a eqp:AircraftType ;
    rdfs:label "Aircraft Type E145"^^xsd:string ;
    eqp:aircraftTypeDesignator "E145"^^xsd:string ;
    eqp:hasAircraftEngineType eqp:JetEngineType ;
    eqp:hasAircraftWeightClass eqp:MediumAircraftWeightClass ;
    eqp:numberOfEngines 2 .

## Airports ############################################################

nas:InternationalAirport a owl:Class ;
    rdfs:label "International airport" ;
    rdfs:comment "The set of international (i.e., non-US) airports." ;
    rdfs:subClassOf nas:Airport .

nas:CONUSairport a owl:Class ;
    rdfs:label "Continental US airport" ;
    rdfs:comment "The set of airports in the continental US." ;
    rdfs:subClassOf nas:USairport .

nas:CanadianAirport a owl:Class ;
    rdfs:label "Canadian airport" ;
    rdfs:comment "The set of Canadian airports." ;
    rdfs:subClassOf nas:InternationalAirport .

nas:airportLocation a owl:FunctionalProperty,
        owl:ObjectProperty ;
    rdfs:label "airport location" ;
    rdfs:comment "Links to a geographic point designated as the airport location." ;
    rdfs:domain nas:Airport ;
    rdfs:range gen:PointLocation .

nas:airportName a owl:DatatypeProperty,
        owl:FunctionalProperty ;
    rdfs:label "airport name" ;
    rdfs:comment "The official name of the airport." ;
    rdfs:domain nas:Airport ;
    rdfs:range xsd:string .

nas:iataAirportCode a owl:DatatypeProperty,
        owl:FunctionalProperty ;
    rdfs:label "IATA Airport Code" ;
    rdfs:comment "The thre-letter IATA code assigned to the airport. Contrast with the ICAO and FAA airport codes." ;
    rdfs:domain nas:Airport ;
    rdfs:range xsd:string .

nas:icaoAirportCode a owl:DatatypeProperty,
        owl:FunctionalProperty ;
    rdfs:label "ICAO airport code" ;
    rdfs:comment "The four-letter ICAO code assignied to the airport. Contrast with the IATA and FAA airport codes." ;
    rdfs:domain nas:Airport ;
    rdfs:range xsd:string .

nas:withinTimezone a owl:DatatypeProperty,
        owl:FunctionalProperty ;
    rdfs:label "within timezone" ;
    rdfs:comment "The timezone identifier for the airport, where the timezone is specified as Area/Location, e.g. America/New_York." ;
    rdfs:domain nas:Airport ;
    rdfs:range xsd:string .

nas:faaAirportCode a owl:DatatypeProperty,
        owl:FunctionalProperty ;
    rdfs:label "FAA airport code" ;
    rdfs:comment "The alphanumeric FAA code of lenth 3 or 4 for the airport. Contrasted with the ICAO and IATA codes, which in general are different. Often the IATA and FAA codes are identical." ;
    rdfs:domain nas:Airport ;
    rdfs:range xsd:string .

nas:locatedInState a owl:DatatypeProperty,
        owl:FunctionalProperty ;
    rdfs:label "Located in State" ;
    rdfs:comment "The 2-letter US postal code for the state in which the airport is located." ;
    rdfs:domain nas:Airport ;
    rdfs:range xsd:string .

nas:withinARTCC a owl:ObjectProperty ;
    rdfs:label "within ARTCC" ;
    rdfs:comment "Links the airport to the ARTCC within which it is located." ;
    rdfs:domain nas:Airport ;
    rdfs:range nas:ARTCC .

nas:withinTimezone a owl:DatatypeProperty,
        owl:FunctionalProperty ;
    rdfs:label "within timezone" ;
    rdfs:comment "The timezone identifier for the airport, where the timezone is specified as Area/Location, e.g. America/New_York." ;
    rdfs:domain nas:Airport ;
    rdfs:range xsd:string .

nas:hoursOffsetFromUTC a owl:DatatypeProperty,
        owl:FunctionalProperty ;
    rdfs:label "hours offset from UTC" ;
    rdfs:comment "The number of hours that the airport is offset from the UTC timezone." ;
    rdfs:domain nas:Airport ;
    rdfs:range xsd:integer .

nas:locatedInState a owl:DatatypeProperty,
        owl:FunctionalProperty ;
    rdfs:label "Located in State" ;
    rdfs:comment "The 2-letter US postal code for the state in which the airport is located." ;
    rdfs:domain nas:Airport ;
    rdfs:range xsd:string .

nas:EGLLairport a nas:InternationalAirport ;                            
    rdfs:label "EGLL Airport"^^xsd:string ;
    nas:airportLocation nas:EGLLcoordinates ;
    nas:airportName "Heathrow"^^xsd:string ;
    nas:iataAirportCode "LHR"^^xsd:string ;
    nas:icaoAirportCode "EGLL"^^xsd:string ;
    nas:withinTimezone "Europe/London"^^xsd:string .

nas:KMIAairport a nas:CONUSairport ;
    rdfs:label "KMIA Airport"^^xsd:string ;
    nas:airportLocation nas:KMIAcoordinates ;
    nas:airportName "MIAMI INTL"^^xsd:string ;
    nas:faaAirportCode "MIA"^^xsd:string ;
    nas:hasRunway nas:KMIAphysicalRunway08L_26R,
        nas:KMIAphysicalRunway08R_26L,
        nas:KMIAphysicalRunway09_27,
        nas:KMIAphysicalRunway12_30 ;
    nas:hoursOffsetFromUTC -5 ;
    nas:iataAirportCode "MIA"^^xsd:string ;
    nas:icaoAirportCode "KMIA"^^xsd:string ;
    nas:locatedInState "FL"^^xsd:string ;
    nas:withinARTCC nas:ZMAcenter ;
    nas:withinTimezone "America/New_York"^^xsd:string .

nas:KDFWairport a nas:CONUSairport ;
    rdfs:label "KDFW Airport"^^xsd:string ;
    nas:airportLocation nas:KDFWcoordinates ;
    nas:airportName "DALLAS/FORT WORTH INTL"^^xsd:string ;
    nas:faaAirportCode "DFW"^^xsd:string ;
    nas:hasRunway nas:KDFWphysicalRunway13L_31R,
        nas:KDFWphysicalRunway13R_31L,
        nas:KDFWphysicalRunway17C_35C,
        nas:KDFWphysicalRunway17L_35R,
        nas:KDFWphysicalRunway17R_35L,
        nas:KDFWphysicalRunway18L_36R,
        nas:KDFWphysicalRunway18R_36L ;
    nas:hasTerminal nas:KDFWtermA,
        nas:KDFWtermB,
        nas:KDFWtermC,
        nas:KDFWtermD,
        nas:KDFWtermE ;
    nas:hoursOffsetFromUTC -6 ;
    nas:iataAirportCode "DFW"^^xsd:string ;
    nas:icaoAirportCode "KDFW"^^xsd:string ;
    nas:locatedInState "TX"^^xsd:string ;
    nas:withinARTCC nas:ZFWcenter ;
    nas:withinTimezone "America/Chicago"^^xsd:string .

nas:KJFKairport a nas:CONUSairport ;
    rdfs:label "KJFK Airport"^^xsd:string ;
    nas:airportLocation nas:KJFKcoordinates ;
    nas:airportName "JOHN F KENNEDY INTL"^^xsd:string ;
    nas:faaAirportCode "JFK"^^xsd:string ;
    nas:hasRunway nas:KJFKphysicalRunway04L_22R,
        nas:KJFKphysicalRunway04R_22L,
        nas:KJFKphysicalRunway13L_31R,
        nas:KJFKphysicalRunway13R_31L ;
    nas:hoursOffsetFromUTC -5 ;
    nas:iataAirportCode "JFK"^^xsd:string ;
    nas:icaoAirportCode "KJFK"^^xsd:string ;
    nas:locatedInState "NY"^^xsd:string ;
    nas:withinARTCC nas:ZNYcenter ;
    nas:withinTimezone "America/New_York"^^xsd:string .

nas:KLGAairport a nas:CONUSairport ;
    rdfs:label "KLGA Airport"^^xsd:string ;
    nas:airportLocation nas:KLGAcoordinates ;
    nas:airportName "LA GUARDIA"^^xsd:string ;
    nas:faaAirportCode "LGA"^^xsd:string ;
    nas:hasRunway nas:KLGAphysicalRunway04_22,
        nas:KLGAphysicalRunway13_31 ;
    nas:hasTerminal nas:KLGAtermA,
        nas:KLGAtermB,
        nas:KLGAtermC,
        nas:KLGAtermD ;
    nas:hoursOffsetFromUTC -5 ;
    nas:iataAirportCode "LGA"^^xsd:string ;
    nas:icaoAirportCode "KLGA"^^xsd:string ;
    nas:locatedInState "NY"^^xsd:string ;
    nas:withinARTCC nas:ZNYcenter ;
    nas:withinTimezone "America/New_York"^^xsd:string . 

nas:KSFOairport a nas:CONUSairport ;
    rdfs:label "KSFO Airport"^^xsd:string ;
    nas:airportLocation nas:KSFOcoordinates ;
    nas:airportName "SAN FRANCISCO INTL"^^xsd:string ;
    nas:faaAirportCode "SFO"^^xsd:string ;
    nas:hasRunway nas:KSFOphysicalRunway01L_19R,
        nas:KSFOphysicalRunway01R_19L,
        nas:KSFOphysicalRunway10L_28R,
        nas:KSFOphysicalRunway10R_28L ;
    nas:hoursOffsetFromUTC -8 ;
    nas:iataAirportCode "SFO"^^xsd:string ;
    nas:icaoAirportCode "KSFO"^^xsd:string ;
    nas:locatedInState "CA"^^xsd:string ;
    nas:withinARTCC nas:ZOAcenter ;
    nas:withinTimezone "America/Los_Angeles"^^xsd:string .   

nas:CYYZairport a nas:CanadianAirport ;
    rdfs:label "CYYZ Airport"^^xsd:string ;
    nas:airportLocation nas:CYYZcoordinates ;
    nas:airportName "TORONTO PEARSON INTL"^^xsd:string ;
    nas:hasRunway nas:CYYZphysicalRunway05_23 ;
    nas:hoursOffsetFromUTC -5 ;
    nas:iataAirportCode "YYZ"^^xsd:string ;
    nas:icaoAirportCode "CYYZ"^^xsd:string ;
    nas:locatedInState "ON"^^xsd:string ;
    nas:withinARTCC nas:CZYcenter ;
    nas:withinTimezone "America/Toronto\r"^^xsd:string .

nas:KEWRairport a nas:CONUSairport ;
    rdfs:label "KEWR Airport"^^xsd:string ;
    nas:airportLocation nas:KEWRcoordinates ;
    nas:airportName "NEWARK LIBERTY INTL"^^xsd:string ;
    nas:faaAirportCode "EWR"^^xsd:string ;
    nas:hasRunway nas:KEWRphysicalRunway04L_22R,
        nas:KEWRphysicalRunway04R_22L,
        nas:KEWRphysicalRunway11_29 ;
    nas:hoursOffsetFromUTC -5 ;
    nas:iataAirportCode "EWR"^^xsd:string ;
    nas:icaoAirportCode "KEWR"^^xsd:string ;
    nas:locatedInState "NJ"^^xsd:string ;
    nas:withinARTCC nas:ZNYcenter ;
    nas:withinTimezone "America/New_York"^^xsd:string .

nas:KSEAairport a nas:CONUSairport ;
    rdfs:label "KSEA Airport"^^xsd:string ;
    nas:airportLocation nas:KSEAcoordinates ;
    nas:airportName "SEATTLE-TACOMA INTL"^^xsd:string ;
    nas:faaAirportCode "SEA"^^xsd:string ;
    nas:hasRunway nas:KSEAphysicalRunway16C_34C,
        nas:KSEAphysicalRunway16L_34R,
        nas:KSEAphysicalRunway16R_34L ;
    nas:hoursOffsetFromUTC -8 ;
    nas:iataAirportCode "SEA"^^xsd:string ;
    nas:icaoAirportCode "KSEA"^^xsd:string ;
    nas:locatedInState "WA"^^xsd:string ;
    nas:withinARTCC nas:ZSEcenter ;
    nas:withinTimezone "America/Los_Angeles"^^xsd:string .

nas:KMHTairport a nas:CONUSairport ;
    rdfs:label "KMHT Airport"^^xsd:string ;
    nas:airportLocation nas:KMHTcoordinates ;
    nas:airportName "MANCHESTER"^^xsd:string ;
    nas:faaAirportCode "MHT"^^xsd:string ;
    nas:hasRunway nas:KMHTphysicalRunway06_24,
        nas:KMHTphysicalRunway17_35 ;
    nas:hoursOffsetFromUTC -5 ;
    nas:iataAirportCode "MHT"^^xsd:string ;
    nas:icaoAirportCode "KMHT"^^xsd:string ;
    nas:locatedInState "NH"^^xsd:string ;
    nas:withinARTCC nas:ZBWcenter ;
    nas:withinTimezone "America/New_York"^^xsd:string .

nas:KCLTairport a nas:CONUSairport ;
    rdfs:label "KCLT Airport"^^xsd:string ;
    nas:airportLocation nas:KCLTcoordinates ;
    nas:airportName "CHARLOTTE/DOUGLAS INTL"^^xsd:string ;
    nas:faaAirportCode "CLT"^^xsd:string ;
    nas:hasRunway nas:KCLTphysicalRunway05_23,
        nas:KCLTphysicalRunway18C_36C,
        nas:KCLTphysicalRunway18L_36R,
        nas:KCLTphysicalRunway18R_36L ;
    nas:hoursOffsetFromUTC -5 ;
    nas:iataAirportCode "CLT"^^xsd:string ;
    nas:icaoAirportCode "KCLT"^^xsd:string ;
    nas:locatedInState "NC"^^xsd:string ;
    nas:withinARTCC nas:ZTLcenter ;
    nas:withinTimezone "America/New_York"^^xsd:string .

## Coordinates #########################################################

nas:EGLLcoordinates a gen:PointLocation ;
    rdfs:label "EGLL coordinates"^^xsd:string ;
    gen:altitude "83"^^xsd:float ;
    gen:latitude "51.477500"^^xsd:float ;
    gen:longitude "-0.461389"^^xsd:float .

nas:KJFKcoordinates a gen:PointLocation ;
    rdfs:label "KJFK coordinates"^^xsd:string ;
    gen:altitude "14"^^xsd:float ;
    gen:latitude "40.639750"^^xsd:float ;
    gen:longitude "-73.778925"^^xsd:float .

nas:KMIAcoordinates a gen:PointLocation ;
    rdfs:label "KMIA coordinates"^^xsd:string ;
    gen:altitude "9"^^xsd:float ;
    gen:latitude "25.795361"^^xsd:float ;
    gen:longitude "-80.290111"^^xsd:float .

nas:KLGAcoordinates a gen:PointLocation ;
    rdfs:label "KLGA coordinates"^^xsd:string ;
    gen:altitude "21"^^xsd:float ;
    gen:latitude "40.777250"^^xsd:float ;
    gen:longitude "-73.872611"^^xsd:float .

nas:KDFWcoordinates a gen:PointLocation ;
    rdfs:label "KDFW coordinates"^^xsd:string ;
    gen:altitude "607"^^xsd:float ;
    gen:latitude "32.897231"^^xsd:float ;
    gen:longitude "-97.037694"^^xsd:float .

nas:KSFOcoordinates a gen:PointLocation ;
    rdfs:label "KSFO coordinates"^^xsd:string ;
    gen:altitude "13"^^xsd:float ;
    gen:latitude "37.619106"^^xsd:float ;
    gen:longitude "-122.375236"^^xsd:float .

nas:CYYZcoordinates a gen:PointLocation ;
    rdfs:label "CYYZ coordinates"^^xsd:string ;
    gen:altitude "569"^^xsd:float ;
    gen:latitude "43.676661"^^xsd:float ;
    gen:longitude "-79.630644"^^xsd:float .

nas:KEWRcoordinates a gen:PointLocation ;
    rdfs:label "KEWR coordinates"^^xsd:string ;
    gen:altitude "18"^^xsd:float ;
    gen:latitude "40.692481"^^xsd:float ;
    gen:longitude "-74.168686"^^xsd:float .

nas:KSEAcoordinates a gen:PointLocation ;
    rdfs:label "KSEA coordinates"^^xsd:string ;
    gen:altitude "433"^^xsd:float ;
    gen:latitude "47.449889"^^xsd:float ;
    gen:longitude "-122.311778"^^xsd:float .

nas:KMHTcoordinates a gen:PointLocation ;
    rdfs:label "KMHT coordinates"^^xsd:string ;
    gen:altitude "266"^^xsd:float ;
    gen:latitude "42.932806"^^xsd:float ;
    gen:longitude "-71.435750"^^xsd:float .

## Actual routes #######################################################

atm:ActualFlightRoute a owl:Class ;
    rdfs:label "Actual Flight Route" ;
    rdfs:comment "A flight trajectory (i.e., a sequence of track points), as determined by flight track surveillance data." ;
    rdfs:subClassOf [ a owl:Restriction ;
            owl:allValuesFrom atm:AircraftTrackPoint ;
            owl:onProperty gen:hasSequencedItem ],
        [ a owl:Restriction ;
            owl:allValuesFrom atm:AircraftTrackPoint ;
            owl:onProperty gen:hasFirstItem ],
        [ a owl:Restriction ;
            owl:allValuesFrom atm:AircraftTrackPoint ;
            owl:onProperty gen:hasLastItem ],
        gen:Sequence .

atm:ActualRouteAAL100-201407150030 a atm:ActualFlightRoute ;
    rdfs:label "Actual Route for AAL100 on 2014-07-15 00:30:00"^^xsd:string ;
    gen:hasFirstItem atm:TrackPt201407150035168241 ;
    gen:hasLastItem atm:TrackPt201407150047159137 ;
    gen:hasSequencedItem atm:TrackPt201407150035168241,
        atm:TrackPt201407150036016540,
        atm:TrackPt201407150036158496,
        atm:TrackPt201407150037033298,
        atm:TrackPt201407150038011997,
        atm:TrackPt201407150038053432,
        atm:TrackPt201407150039016585,
        atm:TrackPt201407150039142779,
        atm:TrackPt201407150040136442,
        atm:TrackPt201407150042003522,
        atm:TrackPt201407150042163295,
        atm:TrackPt201407150044011185,
        atm:TrackPt201407150045036607,
        atm:TrackPt201407150046061041,
        atm:TrackPt201407150047040140,
        atm:TrackPt201407150047159137 .

atm:ActualRouteAAL1102-201407150046 a atm:ActualFlightRoute ;
    rdfs:label "Actual Route for AAL1102 on 2014-07-15 00:46:00"^^xsd:string ;
    gen:hasFirstItem atm:TrackPt201407150052008111 ;
    gen:hasLastItem atm:TrackPt201407150054017098 ;
    gen:hasSequencedItem atm:TrackPt201407150052008111,
        atm:TrackPt201407150052035829,
        atm:TrackPt201407150053030654,
        atm:TrackPt201407150053051356,
        atm:TrackPt201407150054017098 .

atm:ActualRouteAAL1144-201407150040 a atm:ActualFlightRoute ;
    rdfs:label "Actual Route for AAL1144 on 2014-07-15 00:40:00"^^xsd:string ;
    gen:hasFirstItem atm:TrackPt201407150045160390 ;
    gen:hasLastItem atm:TrackPt201407150052117550 ;
    gen:hasSequencedItem atm:TrackPt201407150045160390,
        atm:TrackPt201407150046158584,
        atm:TrackPt201407150047141258,
        atm:TrackPt201407150048111122,
        atm:TrackPt201407150049090586,
        atm:TrackPt201407150050036548,
        atm:TrackPt201407150050088226,
        atm:TrackPt201407150051025266,
        atm:TrackPt201407150051114613,
        atm:TrackPt201407150051133037,
        atm:TrackPt201407150052117349,
        atm:TrackPt201407150052117550 .

atm:ActualRouteAAL1170-201407150053 a atm:ActualFlightRoute ;
    rdfs:label "Actual Route for AAL1170 on 2014-07-15 00:53:00"^^xsd:string ;
    gen:hasFirstItem atm:TrackPt201407150059019717 ;
    gen:hasLastItem atm:TrackPt201407150107104737 ;
    gen:hasSequencedItem atm:TrackPt201407150059019717,
        atm:TrackPt201407150100042224,
        atm:TrackPt201407150100111037,
        atm:TrackPt201407150102075025,
        atm:TrackPt201407150103002879,
        atm:TrackPt201407150103077285,
        atm:TrackPt201407150104129102,
        atm:TrackPt201407150105091434,
        atm:TrackPt201407150105143587,
        atm:TrackPt201407150106115691,
        atm:TrackPt201407150106135668,
        atm:TrackPt201407150107085777,
        atm:TrackPt201407150107104737 .

atm:ActualRouteAAL20-201407152358 a atm:ActualFlightRoute ;
    rdfs:label "Actual Route for AAL20 on 2014-07-15 23:58:00"^^xsd:string ;
    gen:hasFirstItem atm:TrackPt201407160004009387 ;
    gen:hasLastItem atm:TrackPt201407160010120576 ;
    gen:hasSequencedItem atm:TrackPt201407160004009387,
        atm:TrackPt201407160004093371,
        atm:TrackPt201407160005027364,
        atm:TrackPt201407160005117150,
        atm:TrackPt201407160006051030,
        atm:TrackPt201407160006119603,
        atm:TrackPt201407160007075345,
        atm:TrackPt201407160008079906,
        atm:TrackPt201407160009145689,
        atm:TrackPt201407160010120576 .

atm:ActualRouteACA722-201407150025 a atm:ActualFlightRoute ;
    rdfs:label "Actual Route for ACA722 on 2014-07-15 00:25:00"^^xsd:string ;
    gen:hasFirstItem atm:TrackPt201407150031054599 ;
    gen:hasLastItem atm:TrackPt201407150035160163 ;
    gen:hasSequencedItem atm:TrackPt201407150031054599,
        atm:TrackPt201407150031155236,
        atm:TrackPt201407150032160905,
        atm:TrackPt201407150033066739,
        atm:TrackPt201407150033145930,
        atm:TrackPt201407150034063383,
        atm:TrackPt201407150034134237,
        atm:TrackPt201407150035059399,
        atm:TrackPt201407150035160163 .

atm:ActualRouteASA14-201407150005 a atm:ActualFlightRoute ;
    rdfs:label "Actual Route for ASA14 on 2014-07-15 00:05:00"^^xsd:string ;
    gen:hasFirstItem atm:TrackPt201407150010162517 ;
    gen:hasLastItem atm:TrackPt201407150025043901 ;
    gen:hasSequencedItem atm:TrackPt201407150010162517,
        atm:TrackPt201407150012004444,
        atm:TrackPt201407150012159153,
        atm:TrackPt201407150013137273,
        atm:TrackPt201407150014001903,
        atm:TrackPt201407150015044256,
        atm:TrackPt201407150015162929,
        atm:TrackPt201407150017010688,
        atm:TrackPt201407150017143381,
        atm:TrackPt201407150020016149,
        atm:TrackPt201407150021034434,
        atm:TrackPt201407150022040160,
        atm:TrackPt201407150023023639,
        atm:TrackPt201407150024010689,
        atm:TrackPt201407150025043901 .

atm:ActualRouteASQ3831-201407150019 a atm:ActualFlightRoute ;
    rdfs:label "Actual Route for ASQ3831 on 2014-07-15 00:19:00"^^xsd:string ;
    gen:hasFirstItem atm:TrackPt201407150026013204 ;
    gen:hasLastItem atm:TrackPt201407150033008184 ;
    gen:hasSequencedItem atm:TrackPt201407150026013204,
        atm:TrackPt201407150026175968,
        atm:TrackPt201407150027159377,
        atm:TrackPt201407150028146562,
        atm:TrackPt201407150029009441,
        atm:TrackPt201407150030027897,
        atm:TrackPt201407150030046134,
        atm:TrackPt201407150030137356,
        atm:TrackPt201407150031007389,
        atm:TrackPt201407150031173828,
        atm:TrackPt201407150032044449,
        atm:TrackPt201407150033008184 .

atm:ActualRouteASQ4423-201407150037 a atm:ActualFlightRoute ;
    rdfs:label "Actual Route for ASQ4423 on 2014-07-15 00:37:00"^^xsd:string ;
    gen:hasFirstItem atm:TrackPt201407150043108464 ;
    gen:hasLastItem atm:TrackPt201407150055123150 ;
    gen:hasSequencedItem atm:TrackPt201407150043108464,
        atm:TrackPt201407150044075821,
        atm:TrackPt201407150045164562,
        atm:TrackPt201407150046104481,
        atm:TrackPt201407150047089632,
        atm:TrackPt201407150048124841,
        atm:TrackPt201407150049104356,
        atm:TrackPt201407150050154124,
        atm:TrackPt201407150051152091,
        atm:TrackPt201407150052141510,
        atm:TrackPt201407150053111463,
        atm:TrackPt201407150054127641,
        atm:TrackPt201407150055123150 .

atm:ActualRouteCHQ2945-201407150047 a atm:ActualFlightRoute ;
    rdfs:label "Actual Route for CHQ2945 on 2014-07-15 00:47:00"^^xsd:string ;
    gen:hasFirstItem atm:TrackPt201407150053074110 ;
    gen:hasLastItem atm:TrackPt201407150102035883 ;
    gen:hasSequencedItem atm:TrackPt201407150053042977,
        atm:TrackPt201407150053074110,
        atm:TrackPt201407150054073369,
        atm:TrackPt201407150055056700,
        atm:TrackPt201407150056037367,
        atm:TrackPt201407150057041561,
        atm:TrackPt201407150057137003,
        atm:TrackPt201407150059006967,
        atm:TrackPt201407150100030361,
        atm:TrackPt201407150102035883 .

## Planned routes ######################################################

atm:PlannedFlightRoute a owl:Class ;
    rdfs:label "Planned flight route" ;
    rdfs:comment "A planned flight route is an ordered sequence of navigation elements that the pilot intends to traverse en route from origin to destination airport." ;
    rdfs:subClassOf atm:NavigationPath .

atm:flightPlanETA a owl:DatatypeProperty,
        owl:FunctionalProperty ;
    rdfs:label "flight plan ETA" ;
    rdfs:comment "The estimated time of arrival specified in the flight plan." ;
    rdfs:domain atm:PlannedFlightRoute ;
    rdfs:range xsd:dateTime .

atm:flightRouteString a owl:DatatypeProperty,
        owl:FunctionalProperty ;
    rdfs:label "flight route string" ;
    rdfs:comment "A string that provides the route of flight proposed in a flight plan. Syntactically, the string shows a path of fixes, airways, SIDs, and STARs, separated by either one or two dots. The string is parsed to create an equivalent ontology representation: an ordered sequence of navigation elements that are associated directly with the flight plan (atm:PlannedFlightRoute)." ;
    rdfs:domain atm:PlannedFlightRoute ;
    rdfs:range xsd:string .

atm:planFilingDay a owl:FunctionalProperty,
        owl:ObjectProperty ;
    rdfs:label "plan filing day" ;
    rdfs:comment "Links to the day when the flight plan was filed with the FAA." ;
    rdfs:domain atm:PlannedFlightRoute ;
    rdfs:range nas:NASday .

atm:planFilingTime a owl:DatatypeProperty,
        owl:FunctionalProperty ;
    rdfs:label "plan filing time" ;
    rdfs:comment "The time that the flight plan was filed with the FAA." ;
    rdfs:domain atm:PlannedFlightRoute ;
    rdfs:range xsd:dateTime .

atm:planGapAfterSequenceElementNumber a owl:DatatypeProperty ;
    rdfs:label "plan gap after sequence element number" ;
    rdfs:comment "Indicates the location of a gap in the flight plan due to non-parsable/uninterpretable elements in the flight plan string." ;
    rdfs:domain atm:PlannedFlightRoute ;
    rdfs:range xsd:integer .

atm:PlannedRouteAAL100-201407150030 a atm:PlannedFlightRoute ;
    rdfs:label "Planned Route for AAL100 on 2014-07-15 00:30:00"^^xsd:string ;
    atm:flightPlanETA "2014-07-15T06:16:00"^^xsd:dateTime ;
    atm:flightRouteString "KJFK.BETTE3.BETTE..ACK..TUSKY.N271A.TUDEP.NATX.MALOT.NATX.GISTI..SLANY.UL9.STU.UP2.OKESI.Y3.BEDEK..EGLL/0616"^^xsd:string ;
    atm:planFilingDay nas:Day20140714 ;
    atm:planFilingTime "2014-07-14T23:35:46"^^xsd:dateTime .

atm:PlannedRouteAAL1102-201407150046 a atm:PlannedFlightRoute ;
    rdfs:label "Planned Route for AAL1102 on 2014-07-15 00:46:00"^^xsd:string ;
    atm:flightRouteString "KLGA./.EMJAY.J174.WARNN.J174.SWL..CEBEE..WETRO..DIW.AR22.JORAY.HILEY4.KMIA"^^xsd:string ;
    atm:planFilingDay nas:Day20140715 ;
    atm:planFilingTime "2014-07-15T00:46:44"^^xsd:dateTime ;
    atm:planGapAfterSequenceElementNumber "1"^^xsd:Integer ;
    gen:hasFirstItem nas:NEC001_AAL1102-201407150046_KLGA ;
    gen:hasLastItem nas:NEC008_AAL1102-201407150046_KMIA ;
    gen:hasSequencedItem nas:NEC001_AAL1102-201407150046_KLGA,
        nas:NEC002_AAL1102-201407150046_J174,
        nas:NEC003_AAL1102-201407150046_SWL,
        nas:NEC004_AAL1102-201407150046_CEBEE,
        nas:NEC005_AAL1102-201407150046_WETRO,
        nas:NEC006_AAL1102-201407150046_AR22,
        nas:NEC007_AAL1102-201407150046_HILEY4,
        nas:NEC008_AAL1102-201407150046_KMIA .

atm:PlannedRouteAAL1144-201407150040 a atm:PlannedFlightRoute ;
    rdfs:label "Planned Route for AAL1144 on 2014-07-15 00:40:00"^^xsd:string ;
    atm:flightRouteString "KLGA./.MIKYG.Q480.AIR.J80.FYLLS.J29.PXV.J131.LIT.BYP6.KDFW"^^xsd:string ;
    atm:planFilingDay nas:Day20140715 ;
    atm:planFilingTime "2014-07-15T00:42:12"^^xsd:dateTime ;
    atm:planGapAfterSequenceElementNumber "1"^^xsd:Integer ;
    gen:hasFirstItem nas:NEC001_AAL1144-201407150040_KLGA ;
    gen:hasLastItem nas:NEC007_AAL1144-201407150040_KDFW ;
    gen:hasSequencedItem nas:NEC001_AAL1144-201407150040_KLGA,
        nas:NEC002_AAL1144-201407150040_Q480,
        nas:NEC003_AAL1144-201407150040_J80,
        nas:NEC004_AAL1144-201407150040_J29,
        nas:NEC005_AAL1144-201407150040_J131,
        nas:NEC006_AAL1144-201407150040_BYP6,
        nas:NEC007_AAL1144-201407150040_KDFW .

atm:PlannedRouteAAL1170-201407150053 a atm:PlannedFlightRoute ;
    rdfs:label "Planned Route for AAL1170 on 2014-07-15 00:53:00"^^xsd:string ;
    atm:flightRouteString "KDFW.AKUNA4.MLC..RZC..STL..VHP..ROD.J29.DJB..CXR.J146.ETG.MIP4.KLGA"^^xsd:string ;
    atm:planFilingDay nas:Day20140715 ;
    atm:planFilingTime "2014-07-15T00:53:45"^^xsd:dateTime ;
    atm:planGapAfterSequenceElementNumber "0"^^xsd:Integer ;
    gen:hasFirstItem nas:NEC001_AAL1170-201407150053_KDFW ;
    gen:hasLastItem nas:NEC009_AAL1170-201407150053_KLGA ;
    gen:hasSequencedItem nas:NEC001_AAL1170-201407150053_KDFW,
        nas:NEC002_AAL1170-201407150053_AKUNA4,
        nas:NEC003_AAL1170-201407150053_RZC,
        nas:NEC004_AAL1170-201407150053_STL,
        nas:NEC005_AAL1170-201407150053_VHP,
        nas:NEC006_AAL1170-201407150053_J29,
        nas:NEC007_AAL1170-201407150053_J146,
        nas:NEC008_AAL1170-201407150053_MIP4,
        nas:NEC009_AAL1170-201407150053_KLGA .

atm:PlannedRouteAAL20-201407152358 a atm:PlannedFlightRoute ;
    rdfs:label "Planned Route for AAL20 on 2014-07-15 23:58:00"^^xsd:string ;
    atm:flightPlanETA "2014-07-16T05:01:00"^^xsd:dateTime ;
    atm:flightRouteString "KSFO.SHOR5.SAC.J32.BAM.J94.FOD..KG75M..DAFLU..JHW.J70.LVZ.LENDY6.KJFK/0501"^^xsd:string ;
    atm:planFilingDay nas:Day20140716 ;
    atm:planFilingTime "2014-07-16T00:06:41"^^xsd:dateTime ;
    atm:planGapAfterSequenceElementNumber "0"^^xsd:Integer ;
    gen:hasFirstItem nas:NEC001_AAL20-201407152358_KSFO ;
    gen:hasLastItem nas:NEC009_AAL20-201407152358_KJFK ;
    gen:hasSequencedItem nas:NEC001_AAL20-201407152358_KSFO,
        nas:NEC002_AAL20-201407152358_SHOR5,
        nas:NEC003_AAL20-201407152358_J32,
        nas:NEC004_AAL20-201407152358_J94,
        nas:NEC005_AAL20-201407152358_KG75M,
        nas:NEC006_AAL20-201407152358_DAFLU,
        nas:NEC007_AAL20-201407152358_J70,
        nas:NEC008_AAL20-201407152358_LENDY6,
        nas:NEC009_AAL20-201407152358_KJFK .

atm:PlannedRouteACA722-201407150025 a atm:PlannedFlightRoute ;
    rdfs:label "Planned Route for ACA722 on 2014-07-15 00:25:00"^^xsd:string ;
    atm:flightPlanETA "2014-07-15T01:24:00"^^xsd:dateTime ;
    atm:flightRouteString "CYYZ.BULGE2.AIRCO..GEE.GEE111.EXTOL..RKA.HAARP3.KLGA/0124"^^xsd:string ;
    atm:planFilingDay nas:Day20140715 ;
    atm:planFilingTime "2014-07-15T00:25:59"^^xsd:dateTime .

atm:PlannedRouteASA14-201407150005 a atm:PlannedFlightRoute ;
    rdfs:label "Planned Route for ASA14 on 2014-07-15 00:05:00"^^xsd:string ;
    atm:flightPlanETA "2014-07-15T04:48:00"^^xsd:dateTime ;
    atm:flightRouteString "KSEA..SEA.J70.MLP..GTF..HILGR..KP09Y..KP06C..GEP..ODI..KG78K..KG72M..EVOTE..NELLS..KEEHO.J584.SLT.FQM3.KEWR/0448"^^xsd:string ;
    atm:planFilingDay nas:Day20140715 ;
    atm:planFilingTime "2014-07-15T00:24:53"^^xsd:dateTime ;
    atm:planGapAfterSequenceElementNumber "0"^^xsd:Integer ;
    gen:hasFirstItem nas:NEC001_ASA14-201407150005_KSEA ;
    gen:hasLastItem nas:NEC015_ASA14-201407150005_KEWR ;
    gen:hasSequencedItem nas:NEC001_ASA14-201407150005_KSEA,
        nas:NEC002_ASA14-201407150005_J70,
        nas:NEC003_ASA14-201407150005_GTF,
        nas:NEC004_ASA14-201407150005_HILGR,
        nas:NEC005_ASA14-201407150005_KP09Y,
        nas:NEC006_ASA14-201407150005_KP06C,
        nas:NEC007_ASA14-201407150005_GEP,
        nas:NEC008_ASA14-201407150005_ODI,
        nas:NEC009_ASA14-201407150005_KG78K,
        nas:NEC010_ASA14-201407150005_KG72M,
        nas:NEC011_ASA14-201407150005_EVOTE,
        nas:NEC012_ASA14-201407150005_NELLS,
        nas:NEC013_ASA14-201407150005_J584,
        nas:NEC014_ASA14-201407150005_FQM3,
        nas:NEC015_ASA14-201407150005_KEWR .

atm:PlannedRouteASQ3831-201407150019 a atm:PlannedFlightRoute ;
    rdfs:label "Planned Route for ASQ3831 on 2014-07-15 00:19:00"^^xsd:string ;
    atm:flightPlanETA "2014-07-15T01:24:00"^^xsd:dateTime ;
    atm:flightRouteString "CYYZ.BULGE2.AIRCO.V252.GEE.SHAFF7.KEWR/0124"^^xsd:string ;
    atm:planFilingDay nas:Day20140715 ;
    atm:planFilingTime "2014-07-15T00:21:13"^^xsd:dateTime .

atm:PlannedRouteASQ4423-201407150037 a atm:PlannedFlightRoute ;
    rdfs:label "Planned Route for ASQ4423 on 2014-07-15 00:37:00"^^xsd:string ;
    atm:flightPlanETA "2014-07-15T01:41:00"^^xsd:dateTime ;
    atm:flightRouteString "KMHT./.HANAA.FLOSI3.KEWR/0141"^^xsd:string ;
    atm:planFilingDay nas:Day20140715 ;
    atm:planFilingTime "2014-07-15T00:48:21"^^xsd:dateTime ;
    atm:planGapAfterSequenceElementNumber "1"^^xsd:Integer ;
    gen:hasFirstItem nas:NEC001_ASQ4423-201407150037_KMHT ;
    gen:hasLastItem nas:NEC003_ASQ4423-201407150037_KEWR ;
    gen:hasSequencedItem nas:NEC001_ASQ4423-201407150037_KMHT,
        nas:NEC002_ASQ4423-201407150037_FLOSI3,
        nas:NEC003_ASQ4423-201407150037_KEWR .

atm:PlannedRouteCHQ2945-201407150047 a atm:PlannedFlightRoute ;
    rdfs:label "Planned Route for CHQ2945 on 2014-07-15 00:47:00"^^xsd:string ;
    atm:flightRouteString "KJFK./.EMJAY.J174.WARNN.J174.ORF.J121.BARTL.J4.FLO.HUSTN2.KCLT"^^xsd:string ;
    atm:planFilingDay nas:Day20140715 ;
    atm:planFilingTime "2014-07-15T00:47:00"^^xsd:dateTime ;
    atm:planGapAfterSequenceElementNumber "1"^^xsd:Integer ;
    gen:hasFirstItem nas:NEC001_CHQ2945-201407150047_KJFK ;
    gen:hasLastItem nas:NEC006_CHQ2945-201407150047_KCLT ;
    gen:hasSequencedItem nas:NEC001_CHQ2945-201407150047_KJFK,
        nas:NEC002_CHQ2945-201407150047_J174,
        nas:NEC003_CHQ2945-201407150047_J121,
        nas:NEC004_CHQ2945-201407150047_J4,
        nas:NEC005_CHQ2945-201407150047_HUSTN2,
        nas:NEC006_CHQ2945-201407150047_KCLT .

## Airlines ############################################################

nas:AirCarrier a owl:Class ;
    rdfs:label "Air carrier" ;
    rdfs:comment "An entity that it licensed to operate aircraft." ;
    rdfs:subClassOf nas:AviationServiceProvider .

nas:airCarrierName a owl:DatatypeProperty ;
    rdfs:label "Air carrier name" ;
    rdfs:comment "The official name of an air carrier." ;
    rdfs:domain nas:AirCarrier ;
    rdfs:range xsd:string .

nas:airlineCallsign a owl:DatatypeProperty ;
    rdfs:label "airline callsign" ;
    rdfs:comment "The radio call sign associated with an the air carrier. Used by pilots and controllers to identify aircraft over radio frequencies." ;
    rdfs:domain nas:AirCarrier ;
    rdfs:range xsd:string .

nas:countryOfRegistry a owl:DatatypeProperty ;
    rdfs:label "country of registry" ;
    rdfs:comment "The country name of the airline registration." ;
    rdfs:domain nas:AirCarrier ;
    rdfs:range xsd:string .

nas:iataCarrierCode a owl:DatatypeProperty,
        owl:FunctionalProperty ;
    rdfs:label "IATA Carrier Code" ;
    rdfs:comment "The two-letter IATA code assigned to the carrier." ;
    rdfs:domain nas:AirCarrier ;
    rdfs:range xsd:string .

nas:icaoCarrierCode a owl:DatatypeProperty,
        owl:FunctionalProperty ;
    rdfs:label "ICAO Air Carrier Code" ;
    rdfs:comment "The three-letter ICAO code assigned to the airline carrier." ;
    rdfs:domain nas:AirCarrier ;
    rdfs:range xsd:string .

nas:AALairline a nas:AirCarrier ;
    rdfs:label "American Airlines"^^xsd:string ;
    nas:airCarrierName "American Airlines"^^xsd:string ;
    nas:airlineCallsign "AMERICAN"^^xsd:string ;
    nas:countryOfRegistry "United States"^^xsd:string ;
    nas:iataCarrierCode "AA"^^xsd:string ;
    nas:icaoCarrierCode "AAL"^^xsd:string .

nas:ACAairline a nas:AirCarrier ;
    rdfs:label "Air Canada"^^xsd:string ;
    nas:airCarrierName "Air Canada"^^xsd:string ;
    nas:airlineCallsign "AIR CANADA"^^xsd:string ;
    nas:countryOfRegistry "Canada"^^xsd:string ;
    nas:iataCarrierCode "AC"^^xsd:string ;
    nas:icaoCarrierCode "ACA"^^xsd:string .

nas:ASAairline a nas:AirCarrier ;
    rdfs:label "Alaska Airlines"^^xsd:string ;
    nas:airCarrierName "Alaska Airlines"^^xsd:string ;
    nas:airlineCallsign "ALASKA"^^xsd:string ;
    nas:countryOfRegistry "United States"^^xsd:string ;
    nas:iataCarrierCode "AS"^^xsd:string ;
    nas:icaoCarrierCode "ASA"^^xsd:string .

nas:ASQairline a nas:AirCarrier ;
    rdfs:label "Atlantic Southeast Airlines"^^xsd:string ;
    nas:airCarrierName "Atlantic Southeast Airlines"^^xsd:string ;
    nas:airlineCallsign "ACEY"^^xsd:string ;
    nas:countryOfRegistry "United States"^^xsd:string ;
    nas:iataCarrierCode "EV"^^xsd:string ;
    nas:icaoCarrierCode "ASQ"^^xsd:string .

nas:CHQairline a nas:AirCarrier ;
    rdfs:label "Chautauqua Airlines"^^xsd:string ;
    nas:airCarrierName "Chautauqua Airlines"^^xsd:string ;
    nas:airlineCallsign "CHAUTAUQUA"^^xsd:string ;
    nas:countryOfRegistry "United States"^^xsd:string ;
    nas:iataCarrierCode "RP"^^xsd:string ;
    nas:icaoCarrierCode "CHQ"^^xsd:string .
